extraction notes

Clap/leftovers/Phoas_monad.lean
@@ -4,25 +4,14 @@ import Clap.Circuit
 set_option autoImplicit false
 set_option linter.unusedVariables true
 
-namespace Deno
+/-
+  Phoas uses continuations, it may seem natural to look into the continuation monad.
+  However notice that we don't need true continuation, in the sense of returning an arbitrary type, and we don't do any fancy control flow.
+  True continuations seem overkill and additionally we'd need to reason over a Cont monad!
+-/
 
-def eq0 (e:F) : Option Unit :=
-  if e = 0 then some () else none
+namespace Cont_monad
 
-def share (e:F) : F := e
-
-def is_zero (e:F) : F := if e = 0 then 1 else 0
-
-example (i:F) : Option Unit := do
-  let zero := share 0
-  eq0 (zero + i) ;
-  eq0 (zero + i)
-
-end Deno
-
-namespace Phoas_monad
-
--- C the var instance, argument of continuation
 abbrev C var a := Cont (Circuit var) a -- = (a -> Circuit var) -> Circuit var
 
 def lam {var} : C var var := fun k =>
@@ -43,7 +32,13 @@ example {var} : C var Unit := do
   eq0 (.v zero + .v i) ;
   eq0 (.v zero + .v i)
 
-end Phoas_monad
+end Cont_monad
+
+/-
+  We can achieve something similar using just notation.
+  Again, under the notation we still need to reason about
+  continuations, but there is no bind at least.
+-/
 
 namespace Notation
 
@@ -53,10 +48,100 @@ scoped notation "eq0" e => Circuit.eq0 e Circuit.nil
 scoped notation "eq0" e ";" rest => Circuit.eq0 e rest
 scoped notation "let" x ":=" "share" e "in" body => Circuit.share e (fun x => body)
 
-example : Circuit' := fun _ =>
+def x : Circuit' := fun _ =>
   let i := input () in
   let zero := share (.c 0) in
   eq0 (.v zero + .v i) ;
   eq0 (.v zero + .v i)
 
+set_option pp.notation false
+example : x = x := by
+  unfold x
+  sorry
+
 end Notation
+
+/-
+  This is the ideal specification language that we'd like to work with.
+  some () can be seen as true and none as false, using Option α
+  however allows functions to return more interesting things than ().
+-/
+
+namespace Spec
+
+def eq0 (e:F) : Option Unit :=
+  if e = 0 then some () else none
+
+-- just the identity
+def share (e:F) : F := e
+
+def is_zero (e:F) : F := if e = 0 then 1 else 0
+
+/-
+  A circuit is a function from any number of F arguments to Option Unit.
+-/
+
+def ex (i:F) : Option Unit := do
+  let zero := share 0
+  eq0 (zero + i)
+  eq0 (zero + i)
+
+end Spec
+
+/-
+  Our Circuit type has its own `denotation` which is different than Option Unit.
+  We can however take a denotation and map it to a corresponding Spec type.
+-/
+
+def deno2spec (d:denotation) : Type :=
+  match d with
+  | .u => Option Unit
+  | .n => Option Unit
+  | .l f => (x:F) -> deno2spec (f x)
+
+/-
+  Now we can define a notion of equivalence between our Spec programs and the denotation of our Circuits.
+-/
+
+inductive s_bisim : (l: denotation) -> (r:deno2spec l) -> Prop where
+  | none
+      : s_bisim .n none
+  | unit
+      : s_bisim .u (some ())
+  | lam
+      (kl:F -> denotation)
+      (kr:deno2spec (.l kl))
+      (h: ∀ x, s_bisim (kl x) (kr x))
+      : s_bisim (.l kl) kr
+
+notation : 65 t:65 "≡" s:66 => s_bisim t s
+
+/-
+  Given a Source program, there exists a denotation that is equivalent to it.
+  - We just have to find it -
+-/
+
+example : ∃ (c:Circuit'), eval' c ≡ Spec.ex := by
+/-
+  eval' ?c ≡ ex
+unfold eval'
+  eval (?d F) ≡ ex
+era-espand
+  eval ((fun var => ?e) F) ≡ ex
+simp
+  eval ?f ≡ ex
+unfold ex, ?f can only be a .lam
+  eval (.lam ?k) ≡ fun i => rest
+simp eval
+  .l (fun x -> eval (?k x)) ≡ fun i => rest
+s_bisim.lam
+  ∀ x, eval (?k x) ≡ rest
+unfold rest right to left
+  eval ((fun y => ?g (eq0 (zero + x) nil)) x) ≡ rest' ; eq0 (zero+x)
+unfold rest right to left
+  eval ((fun y => ?h (eq0 (zero + x) (eq0 (zero + x) nil)) x) ≡ rest'' ; eq0 (zero+x) ; eq0 (zero+x)
+  eval ((fun y => share (.c 0) (fun zero -> (eq0 (zero + x) (eq0 (zero + x) nil)))) x) ≡ let zero = share 0 ; eq0 (zero+x) ; eq0 (zero+x)
+
+-/
+
+  sorry
